more stuff

SSA/Experimental/Bits/Defs.lean
@@ -1,4 +1,5 @@
 import Mathlib.Data.Bool.Basic
+import Mathlib.Data.Fin.Basic
 
 inductive Term : Type
 | var : Nat → Term
@@ -9,7 +10,7 @@ inductive Term : Type
 | or : Term → Term → Term
 | xor : Term → Term → Term
 | not : Term → Term
-| ls : Term → Term
+| ls (b : Bool) : Term → Term
 | add : Term → Term → Term
 | sub : Term → Term → Term
 | neg : Term → Term
@@ -20,7 +21,7 @@ open Term
 
 def zeroSeq : Nat → Bool := fun _ => false
 
-def oneSeq : Nat → Bool := fun n => n == 0
+def oneSeq : Nat → Bool := fun n => n = 0
 
 def negOneSeq : Nat → Bool := fun _ => true
 
@@ -32,8 +33,8 @@ def xorSeq : ∀ (_ _ : Nat → Bool), Nat → Bool := fun x y n => xor (x n) (y
 
 def notSeq : ∀ (_ : Nat → Bool), Nat → Bool := fun x n => !(x n)
 
-def lsSeq (s : Nat → Bool) : Nat → Bool
-  | 0 => false
+def lsSeq (b : Bool) (s : Nat → Bool) : Nat → Bool
+  | 0 => b 
   | (n+1) => s n
 
 def addSeqAux (x y : Nat → Bool) : Nat → Bool × Bool
@@ -97,7 +98,7 @@ def Term.eval : ∀ (_ : Term) (_ : Nat → Nat → Bool), Nat → Bool
 | or t₁ t₂, vars => orSeq (Term.eval t₁ vars) (Term.eval t₂ vars)
 | xor t₁ t₂, vars => xorSeq (Term.eval t₁ vars) (Term.eval t₂ vars)
 | not t, vars => notSeq (Term.eval t vars)
-| ls t, vars => lsSeq (Term.eval t vars)
+| ls b t, vars => lsSeq b (Term.eval t vars)
 | add t₁ t₂, vars => addSeq (Term.eval t₁ vars) (Term.eval t₂ vars)
 | sub t₁ t₂, vars => subSeq (Term.eval t₁ vars) (Term.eval t₂ vars)
 | neg t, vars => negSeq (Term.eval t vars)
@@ -109,4 +110,56 @@ instance : Sub Term := ⟨sub⟩
 instance : One Term := ⟨one⟩
 instance : Zero Term := ⟨zero⟩
 instance : Neg Term := ⟨neg⟩
+
+@[simp] def Term.arity : Term → ℕ
+| (var n) => n+1
+| zero => 0
+| one => 0
+| negOne => 0
+| Term.and t₁ t₂ => max (arity t₁) (arity t₂)
+| Term.or t₁ t₂ => max (arity t₁) (arity t₂)
+| Term.xor t₁ t₂ => max (arity t₁) (arity t₂)
+| Term.not t => arity t
+| ls _ t => arity t
+| add t₁ t₂ => max (arity t₁) (arity t₂)
+| sub t₁ t₂ => max (arity t₁) (arity t₂)
+| neg t => arity t
+| incr t => arity t
+| decr t => arity t
+
+@[simp] def Term.evalFin : ∀ (t : Term) (_vars : Fin (arity t) → ℕ → Bool), ℕ → Bool
+| var n, vars => vars (Fin.last n)
+| zero, _vars => zeroSeq
+| one, _vars => oneSeq
+| negOne, _vars => negOneSeq
+| Term.and t₁ t₂, vars =>
+  andSeq (Term.evalFin t₁
+    (fun i => vars (Fin.castLE (by simp [arity]) i)))
+  (Term.evalFin t₂
+    (fun i => vars (Fin.castLE (by simp [arity]) i)))
+| Term.or t₁ t₂, vars =>
+  orSeq (Term.evalFin t₁
+    (fun i => vars (Fin.castLE (by simp [arity]) i)))
+  (Term.evalFin t₂
+    (fun i => vars (Fin.castLE (by simp [arity]) i)))
+| Term.xor t₁ t₂, vars =>
+  xorSeq (Term.evalFin t₁
+    (fun i => vars (Fin.castLE (by simp [arity]) i)))
+  (Term.evalFin t₂
+    (fun i => vars (Fin.castLE (by simp [arity]) i)))
+| not t, vars => notSeq (Term.evalFin t vars)
+| ls b t, vars => lsSeq b (Term.evalFin t vars)
+| add t₁ t₂, vars =>
+  addSeq (Term.evalFin t₁
+    (fun i => vars (Fin.castLE (by simp [arity]) i)))
+  (Term.evalFin t₂
+    (fun i => vars (Fin.castLE (by simp [arity]) i)))
+| sub t₁ t₂, vars =>
+  subSeq (Term.evalFin t₁
+    (fun i => vars (Fin.castLE (by simp [arity]) i)))
+  (Term.evalFin t₂
+    (fun i => vars (Fin.castLE (by simp [arity]) i)))
+| neg t, vars => negSeq (Term.evalFin t vars)
+| incr t, vars => incrSeq (Term.evalFin t vars)
+| decr t, vars => decrSeq (Term.evalFin t vars)
 
