SSA/Experimental/Bits/Fast/FiniteStateMachine.lean
@@ -38,6 +38,11 @@ def eval (x : arity → ℕ → Bool) : ℕ → Bool :=
 def carry (x : arity → ℕ → Bool) : ℕ → p.α → Bool :=
   fun n => (evalAux p x n).1
 
+theorem eval_eq_carry (x : arity → ℕ → Bool) (n : ℕ) : 
+  p.eval x n = (p.next_bit (Nat.casesOn n p.init_carry (p.carry x)) 
+    (fun i => x i n)).2 := by
+  cases n <;> rfl
+
 def changeVars {arity2 : Type} (changeVars : arity → arity2) :
     FSM arity2 :=
   { α := p.α,
@@ -85,7 +90,7 @@ lemma evalAux_compose [Fintype arity]
   | 0 => by
       ext y
       cases y
-      . simp [evalAux, next_bit, compose, Circuit.eval_bind, eval]
+      . simp only [evalAux, next_bit, compose, Circuit.eval_bind, eval]
         congr
         ext z
         cases z
@@ -146,183 +151,288 @@ lemma evalAux_compose [Fintype arity]
           . simp
           . simp       
 
+lemma eval_compose [Fintype arity]
+    (new_arity : Type)
+    (q_arity : arity → Type)
+    (vars : ∀ (a : arity), q_arity a → new_arity)
+    (q : ∀ (a : arity), FSM (q_arity a))
+    (x : new_arity → ℕ → Bool) :
+    (p.compose new_arity q_arity vars q).eval x = 
+      p.eval (λ a => (q a).eval (fun i => x (vars _ i))) := by
+  ext n
+  rw [eval, evalAux_compose, eval]
 
 def and : FSM Bool :=
   { α := Empty,
     i := by infer_instance,
     init_carry := Empty.elim,
-    next_bit := λ _carry bits => (Empty.elim, bits true && bits false) }
+    next_bit_circ := fun a => a.elim 
+      (Circuit.and 
+        (Circuit.var true (inr true)) 
+        (Circuit.var true (inr false))) Empty.elim }
 
 @[simp] lemma eval_and (x : Bool → ℕ → Bool) : and.eval x = andSeq (x true) (x false) := by
-  ext n; cases n <;> simp [and, andSeq, eval, propagate_succ]
+  ext n; cases n <;> simp [and, andSeq, evalAux, eval, next_bit]
 
 def or : FSM Bool :=
   { α := Empty,
     i := by infer_instance,
     init_carry := Empty.elim,
-    next_bit := λ _carry bits => (Empty.elim, bits true || bits false) }
+    next_bit_circ := fun a => a.elim 
+      (Circuit.or 
+        (Circuit.var true (inr true)) 
+        (Circuit.var true (inr false))) Empty.elim }
 
 @[simp] lemma eval_or (x : Bool → ℕ → Bool) : or.eval x = orSeq (x true) (x false) := by
-  ext n; cases n <;> simp [or, orSeq, eval, propagate_succ]
+  ext n; cases n <;> simp [and, orSeq, evalAux, eval, next_bit]
 
 def xor : FSM Bool :=
   { α := Empty,
     i := by infer_instance,
     init_carry := Empty.elim,
-    next_bit := λ _carry bits => (Empty.elim, _root_.xor (bits true) (bits false)) }
+    next_bit_circ := fun a => a.elim 
+      (Circuit.xor 
+        (Circuit.var true (inr true)) 
+        (Circuit.var true (inr false))) Empty.elim }
 
 @[simp] lemma eval_xor (x : Bool → ℕ → Bool) : xor.eval x = xorSeq (x true) (x false) := by
-  ext n; cases n <;> simp [xor, xorSeq, eval, propagate_succ]
+  ext n; cases n <;> simp [and, xorSeq, evalAux, eval, next_bit]
 
-  def add : FSM Bool :=
+def add : FSM Bool :=
   { α := Unit,
     i := by infer_instance,
     init_carry := λ _ => false,
-    next_bit := λ (carry : Unit → Bool) (bits : Bool → Bool) =>
-        (λ _ => (bits true && bits false) || (bits false && carry ()) || (bits true && carry ()),
-          _root_.xor (bits true) (_root_.xor (bits false) (carry ()))) }
+    next_bit_circ := fun a =>
+      match a with
+      | some () => 
+             (Circuit.var true (inr true) &&& Circuit.var true (inr false)) |||
+             (Circuit.var true (inr false) &&& Circuit.var true (inl ())) |||
+             (Circuit.var true (inr true) &&& Circuit.var true (inl ()))
+      | none => Circuit.var true (inr true) ^^^ 
+                Circuit.var true (inr false) ^^^ 
+                Circuit.var true (inl ()) }
+
+theorem evalAux_add (x : Bool → ℕ → Bool) : ∀ (n : ℕ), add.evalAux x n = 
+    (fun _ => (addSeqAux (x true) (x false) n).2, (addSeqAux (x true) (x false) n).1)
+  | 0 => by
+    simp [evalAux, next_bit, Function.funext_iff, addSeqAux, add]
+  | n+1 => by
+    rw [evalAux, evalAux_add _ n]
+    simp [next_bit, Function.funext_iff, addSeqAux]
 
 @[simp] lemma eval_add (x : Bool → ℕ → Bool) : add.eval x = addSeq (x true) (x false) := by
-  dsimp [add, eval]
-  rw [add_eq_propagate]
-  congr
-  funext b
-  cases b; rfl
-  simp
-  congr
-  funext i
-  cases i <;> simp
-
+  ext n
+  rw [eval, evalAux_add]; rfl
 
 def sub : FSM Bool :=
   { α := Unit,
     i := by infer_instance,
     init_carry := λ _ => false,
-    next_bit := λ (carry : Unit → Bool) (bits : Bool → Bool) =>
-        (λ _ => (!(bits true) && (bits false)) ||
-          ((!(_root_.xor (bits true) (bits false))) && carry ()),
-          _root_.xor (bits true) (_root_.xor (bits false) (carry ()))) }
+    next_bit_circ := fun a =>
+      match a with
+      | some () => 
+             (Circuit.var false (inr true) &&& Circuit.var true (inr false)) |||
+             ((Circuit.var false (inr true) ^^^ Circuit.var true (inr false)) &&&
+              (Circuit.var true (inl ())))
+      | none => Circuit.var true (inr true) ^^^ 
+                Circuit.var true (inr false) ^^^ 
+                Circuit.var true (inl ()) }
+
+theorem evalAux_sub (x : Bool → ℕ → Bool) : ∀ (n : ℕ), sub.evalAux x n = 
+    (fun _ => (subSeqAux (x true) (x false) n).2, (subSeqAux (x true) (x false) n).1)
+  | 0 => by
+    simp [evalAux, next_bit, Function.funext_iff, subSeqAux, sub]
+  | n+1 => by
+    rw [evalAux, evalAux_sub _ n]
+    simp [next_bit, Function.funext_iff, subSeqAux, Bool.xor_not_left']
 
 @[simp] lemma eval_sub (x : Bool → ℕ → Bool) : sub.eval x = subSeq (x true) (x false) := by
-  dsimp [sub, eval]
-  rw [sub_eq_propagate]
-  congr
-  funext b
-  cases b;  rfl
-  simp
-  congr
-  funext i
-  cases i <;> simp
+  ext n
+  rw [eval, evalAux_sub]; rfl
 
 def neg : FSM Unit :=
   { α := Unit,
     i := by infer_instance,
     init_carry := λ _ => true,
-    next_bit := λ (carry : Unit → Bool) (bits : Unit → Bool) =>
-      (λ _ => (!(bits ())) && (carry ()), _root_.xor (!(bits ())) (carry ())) }
+    next_bit_circ := fun a =>
+      match a with
+      | some () => Circuit.var false (inr ()) &&& Circuit.var true (inl ())
+      | none => Circuit.var false (inr ()) ^^^ Circuit.var true (inl ())  }
+
+theorem evalAux_neg (x : Unit → ℕ → Bool) : ∀ (n : ℕ), neg.evalAux x n = 
+    (fun _ => (negSeqAux (x ()) n).2, (negSeqAux (x ()) n).1)
+  | 0 => by
+    simp [evalAux, next_bit, Function.funext_iff, negSeqAux, neg]
+  | n+1 => by
+    rw [evalAux, evalAux_neg _ n]
+    simp [next_bit, Function.funext_iff, negSeqAux, Bool.xor_not_left']
 
 @[simp] lemma eval_neg (x : Unit → ℕ → Bool) : neg.eval x = negSeq (x ()) := by
-  dsimp [neg, eval]
-  rw [neg_eq_propagate]
+  ext n
+  rw [eval, evalAux_neg]; rfl
 
 def not : FSM Unit :=
-{ α := Empty,
-  i := by infer_instance,
-  init_carry := Empty.elim,
-  next_bit := λ _carry bits => (Empty.elim, !(bits ())) }
+  { α := Empty,
+    i := by infer_instance,
+    init_carry := Empty.elim,
+    next_bit_circ := fun _ => Circuit.var false (inr ()) }
 
 @[simp] lemma eval_not (x : Unit → ℕ → Bool) : not.eval x = notSeq (x ()) := by
-  ext n; cases n <;> simp [not, notSeq, eval, propagate_succ]
+  ext n; cases n <;> simp [eval, evalAux, not, notSeq, next_bit]
 
 def zero : FSM (Fin 0) :=
   { α := Empty,
     i := by infer_instance,
     init_carry := Empty.elim,
-    next_bit := λ _carry _bits => (Empty.elim, false) }
+    next_bit_circ := fun _ => Circuit.fals }
 
 @[simp] lemma eval_zero (x : Fin 0 → ℕ → Bool) : zero.eval x = zeroSeq := by
-  ext n; cases n <;> simp [zero, zeroSeq, eval, propagate_succ]
+  ext n; cases n <;> simp [zero, zeroSeq, eval, next_bit, evalAux]
 
 def one : FSM (Fin 0) :=
   { α := Unit,
     i := by infer_instance,
     init_carry := λ _ => true,
-    next_bit := λ carry _bits => (λ _ => false, carry ()) }
+    next_bit_circ := fun a => 
+      match a with
+      | some () => Circuit.fals
+      | none => Circuit.var true (inl ()) }
+
+theorem evalAux_one (x : Fin 0 → ℕ → Bool) : ∀ (n : ℕ),
+    one.evalAux x n = (fun _ => false, oneSeq n) 
+  | 0 => by simp [evalAux, next_bit, one, oneSeq]
+  | n+1 => by 
+    rw [evalAux, evalAux_one _ n]
+    simp [next_bit, oneSeq]
 
 @[simp] lemma eval_one (x : Fin 0 → ℕ → Bool) : one.eval x = oneSeq := by
-  ext n; cases n <;> simp [one, oneSeq, eval, propagate_succ2, @eq_comm _ false]
+  ext n
+  rw [eval, evalAux_one]
 
 def negOne : FSM (Fin 0) :=
   { α := Empty,
     i := by infer_instance,
     init_carry := Empty.elim,
-    next_bit := λ _carry _bits => (Empty.elim, true) }
+    next_bit_circ := fun _ => Circuit.tru }
 
 @[simp] lemma eval_negOne (x : Fin 0 → ℕ → Bool) : negOne.eval x = negOneSeq := by
-  ext n; cases n <;> simp [negOne, negOneSeq, eval, propagate_succ2]
+  ext n; cases n <;> simp [negOne, negOneSeq, eval, evalAux, next_bit]
 
-def ls : FSM Unit :=
+def ls (b : Bool) : FSM Unit :=
   { α := Unit,
     i := by infer_instance,
-    init_carry := λ _ => false,
-    next_bit := λ carry bits => (bits, carry ()) }
+    init_carry := λ _ => b,
+    next_bit_circ := fun x => 
+      match x with
+      | none => Circuit.var true (inl ())
+      | some () => Circuit.var true (inr ()) }
 
-@[simp] lemma eval_ls (x : Unit → ℕ → Bool) : ls.eval x = lsSeq (x ()) := by
-  ext n; cases n <;> simp [ls, lsSeq, eval, propagate_succ2]
+theorem evalAux_ls (b : Bool) (x : Unit → ℕ → Bool) : ∀ (n : ℕ),
+    (ls b).evalAux x n = (fun _ => x () n, lsSeq b (x ()) n)
+  | 0 => by simp [evalAux, next_bit, ls, lsSeq]
+  | n+1 => by
+    rw [evalAux, evalAux_ls _ _ n]
+    simp [next_bit, lsSeq]
+
+@[simp] lemma eval_ls (b : Bool) (x : Unit → ℕ → Bool) : (ls b).eval x = lsSeq b (x ()) := by
+  ext n
+  rw [eval, evalAux_ls]
 
 def var (n : ℕ) : FSM (Fin (n+1)) :=
   { α := Empty,
     i := by infer_instance,
     init_carry := Empty.elim,
-    next_bit := λ _carry bits => (Empty.elim, bits (Fin.last n)) }
+    next_bit_circ := λ _ => Circuit.var true (inr (Fin.last _)) }
 
 @[simp] lemma eval_var (n : ℕ) (x : Fin (n+1) → ℕ → Bool) : (var n).eval x = x (Fin.last n) := by
-  ext m; cases m <;> simp [var, eval, propagate_succ]
+  ext m; cases m <;> simp [var, eval, evalAux, next_bit]
 
 def incr : FSM Unit :=
   { α := Unit,
     i := by infer_instance,
     init_carry := λ _ => true,
-    next_bit := λ carry bits => (λ _ => bits () && carry (), _root_.xor (bits ()) (carry ())) }
+    next_bit_circ := fun x => 
+      match x with
+      | none => (Circuit.var true (inr ())) ^^^ (Circuit.var true (inl ()))
+      | some _ => (Circuit.var true (inr ())) &&& (Circuit.var true (inl ())) }
+
+theorem evalAux_incr (x : Unit → ℕ → Bool) : ∀ n, 
+    incr.evalAux x n = (fun _ => (incrSeqAux (x ()) n).2, (incrSeqAux (x ()) n).1)
+  | 0 => by simp [evalAux, next_bit, next_bit, incrSeqAux, incr]
+  | n+1 => by
+    rw [evalAux, evalAux_incr _ n]
+    simp [next_bit, incrSeqAux, incr]
 
 @[simp] lemma eval_incr (x : Unit → ℕ → Bool) : incr.eval x = incrSeq (x ()) := by
-  dsimp [incr, eval]
-  rw [incr_eq_propagate]
+  ext n
+  rw [eval, evalAux_incr]; rfl
 
 def decr : FSM Unit :=
   { α := Unit,
     i := by infer_instance,
     init_carry := λ _ => true,
-    next_bit := λ carry bits => (λ _ => !(bits ()) && carry (), _root_.xor (bits ()) (carry ())) }
+    next_bit_circ := fun x => 
+      match x with
+      | none => (Circuit.var true (inr ())) ^^^ (Circuit.var true (inl ()))
+      | some _ => (Circuit.var false (inr ())) &&& (Circuit.var true (inl ())) }
+
+theorem evalAux_decr (x : Unit → ℕ → Bool) : ∀ n, 
+    decr.evalAux x n = (fun _ => (decrSeqAux (x ()) n).2, (decrSeqAux (x ()) n).1)
+  | 0 => by simp [evalAux, next_bit, next_bit, decrSeqAux, decr]
+  | n+1 => by
+    rw [evalAux, evalAux_decr _ n]
+    simp [next_bit, decrSeqAux, decr]
 
 @[simp] lemma eval_decr (x : Unit → ℕ → Bool) : decr.eval x = decrSeq (x ()) := by
-  dsimp [decr, eval]
-  rw [decr_eq_propagate]
+  ext n
+  rw [eval, evalAux_decr]; rfl
+
+theorem evalAux_eq_zero_of_set {arity : Type _} (p : FSM arity) 
+    (R : Set (p.α → Bool)) (hR : ∀ x s, (p.next_bit s x).1 ∈ R → s ∈ R) 
+    (hi : p.init_carry ∉ R) (hr1 : ∀ x s, (p.next_bit s x).2 = true → s ∈ R)
+    (x : arity → ℕ → Bool) (n : ℕ) : p.eval x n = false ∧ p.carry x n ∉ R := by
+  simp (config := {singlePass := true}) only [← not_imp_not] at hR hr1
+  simp only [Bool.not_eq_true] at hR hr1
+  induction n with
+  | zero => 
+    simp only [eval, evalAux, carry]
+    exact ⟨hr1 _ _ hi, hR _ _ hi⟩
+  | succ n ih => 
+    simp only [eval, evalAux, carry] at ih ⊢
+    exact ⟨hr1 _ _ ih.2, hR _ _ ih.2⟩ 
+
+theorem eval_eq_zero_of_set {arity : Type _} (p : FSM arity) 
+    (R : Set (p.α → Bool)) (hR : ∀ x s, (p.next_bit s x).1 ∈ R → s ∈ R) 
+    (hi : p.init_carry ∉ R) (hr1 : ∀ x s, (p.next_bit s x).2 = true → s ∈ R) :
+    p.eval = fun _ _ => false := by
+  ext x n
+  rw [eval]
+  exact (evalAux_eq_zero_of_set p R hR hi hr1 x n).1
 
 end FSM
 
-structure PropagateSolution (t : Term) extends FSM (Fin (arity t)) :=
+structure FSMSolution (t : Term) extends FSM (Fin t.arity) :=
 ( good : t.evalFin = toFSM.eval )
 
 def composeUnary
     (p : FSM Unit)
     {t : Term}
-    (q : PropagateSolution t) :
-    FSM (Fin (arity t)) :=
+    (q : FSMSolution t) :
+    FSM (Fin t.arity) :=
   p.compose
-    (Fin (arity t))
+    (Fin t.arity)
     _
     (λ _ => id)
     (λ _ => q.toFSM)
-def X := @Bool.casesOn
+
 def composeBinary
     (p : FSM Bool)
     {t₁ t₂ : Term}
-    (q₁ : PropagateSolution t₁)
-    (q₂ : PropagateSolution t₂) :
-    FSM (Fin (max (arity t₁) (arity t₂))) :=
-  p.compose (Fin (max (arity t₁) (arity t₂)))
-    (λ b => Fin (cond b (arity t₁) (arity t₂)))
+    (q₁ : FSMSolution t₁)
+    (q₂ : FSMSolution t₂) :
+    FSM (Fin (max t₁.arity t₂.arity)) :=
+  p.compose (Fin (max t₁.arity t₂.arity))
+    (λ b => Fin (cond b t₁.arity t₂.arity))
     (λ b i => Fin.castLE (by cases b <;> simp) i)
     (λ b => match b with
       | true => q₁.toFSM
@@ -331,17 +441,17 @@ def composeBinary
 @[simp] lemma composeUnary_eval
     (p : FSM Unit)
     {t : Term}
-    (q : PropagateSolution t)
-    (x : Fin (arity t) → ℕ → Bool) :
+    (q : FSMSolution t)
+    (x : Fin t.arity → ℕ → Bool) :
     (composeUnary p q).eval x = p.eval (λ _ => t.evalFin x) := by
   rw [composeUnary, FSM.eval_compose, q.good]; rfl
 
 @[simp] lemma composeBinary_eval
     (p : FSM Bool)
     {t₁ t₂ : Term}
-    (q₁ : PropagateSolution t₁)
-    (q₂ : PropagateSolution t₂)
-    (x : Fin (max (arity t₁) (arity t₂)) → ℕ → Bool) :
+    (q₁ : FSMSolution t₁)
+    (q₂ : FSMSolution t₂)
+    (x : Fin (max t₁.arity t₂.arity) → ℕ → Bool) :
     (composeBinary p q₁ q₂).eval x = p.eval
       (λ b => cond b (t₁.evalFin (fun i => x (Fin.castLE (by simp) i)))
                   (t₂.evalFin (fun i => x (Fin.castLE (by simp) i)))) := by
@@ -351,290 +461,67 @@ def composeBinary
   cases b <;> dsimp <;> congr <;> funext b <;> cases b <;> simp
 
 instance {α β : Type} [Fintype α] [Fintype β] (b : Bool) :
-    Fintype (cond b α β) :=
-  by cases b <;> simp <;> infer_instance
+    Fintype (cond b α β) := by
+  cases b <;> simp <;> infer_instance
 
-lemma cond_propagate {α α' β β' : Type}
-    (init_carry : α → Bool)
-    (next_bit : ∀ (_carry : α → Bool) (_bits : β → Bool),
-      (α → Bool) × Bool)
-    (init_carry' : α' → Bool)
-    (next_bit' : ∀ (_carry : α' → Bool) (_bits : β' → Bool),
-      (α' → Bool) × Bool)
-    {γ : Type} (fβ : β → γ) (fβ' : β' → γ)
-    (x : γ → ℕ → Bool) (b : Bool) :
-    cond b (propagate init_carry next_bit (λ b => (x (fβ b))))
-      (propagate init_carry' next_bit' (λ b => (x (fβ' b)))) =
-    propagate (show cond b α α' → Bool from Bool.rec init_carry' init_carry b)
-      (show ∀ (_carry : cond b α α' → Bool) (_bits : cond b β β' → Bool),
-          (cond b α α' → Bool) × Bool
-        from Bool.rec next_bit' next_bit b)
-      (show cond b β β' → ℕ → Bool from Bool.rec (λ b => (x (fβ' b))) (λ b => (x (fβ b))) b) :=
-  by cases b <;> rfl
+open Term
 
-def termEvalEqPropagate : ∀ (t : Term),
-  PropagateSolution t
-| var n =>
-  { toFSM := FSM.var n,
-    good := by ext; simp [Term.evalFin] }
-| zero =>
-  { toFSM := FSM.zero,
-    good := by ext; simp [Term.evalFin] }
-| one =>
-  { toFSM := FSM.one,
-    good := by ext; simp [Term.evalFin] }
-| negOne =>
-  { toFSM := FSM.negOne,
-    good := by ext; simp [Term.evalFin] }
-| Term.and t₁ t₂ =>
-  let q₁ := termEvalEqPropagate t₁
-  let q₂ := termEvalEqPropagate t₂
-  { toFSM := composeBinary FSM.and q₁ q₂,
-    good := by ext; simp }
-| Term.or t₁ t₂ =>
-  let q₁ := termEvalEqPropagate t₁
-  let q₂ := termEvalEqPropagate t₂
-  { toFSM := composeBinary FSM.or q₁ q₂,
-    good := by ext; simp }
-| Term.xor t₁ t₂ =>
-  let q₁ := termEvalEqPropagate t₁
-  let q₂ := termEvalEqPropagate t₂
-  { toFSM := composeBinary FSM.xor q₁ q₂,
-    good := by ext; simp }
-| ls t =>
-  let q := termEvalEqPropagate t
-  { toFSM := by dsimp [arity]; exact composeUnary FSM.ls q,
-    good := by ext; simp }
-| Term.not t =>
-  let q := termEvalEqPropagate t
-  { toFSM := by dsimp [arity]; exact composeUnary FSM.not q,
-    good := by ext; simp }
-| add t₁ t₂ =>
-  let q₁ := termEvalEqPropagate t₁
-  let q₂ := termEvalEqPropagate t₂
-  { toFSM := composeBinary FSM.add q₁ q₂,
-    good := by ext; simp }
-| sub t₁ t₂ =>
-  let q₁ := termEvalEqPropagate t₁
-  let q₂ := termEvalEqPropagate t₂
-  { toFSM := composeBinary FSM.sub q₁ q₂,
-    good := by ext; simp }
-| neg t =>
-  let q := termEvalEqPropagate t
-  { toFSM := by dsimp [arity]; exact composeUnary FSM.neg q,
-    good := by ext; simp }
-| incr t =>
-  let q := termEvalEqPropagate t
-  { toFSM := by dsimp [arity]; exact composeUnary FSM.incr q,
-    good := by ext; simp }
-| decr t =>
-  let q := termEvalEqPropagate t
-  { toFSM := by dsimp [arity]; exact composeUnary FSM.decr q,
-    good := by ext; simp }
+def termEvalEqFSM : ∀ (t : Term), FSMSolution t
+  | var n =>
+    { toFSM := FSM.var n,
+      good := by ext; simp [Term.evalFin] }
+  | zero =>
+    { toFSM := FSM.zero,
+      good := by ext; simp [Term.evalFin] }
+  | one =>
+    { toFSM := FSM.one,
+      good := by ext; simp [Term.evalFin] }
+  | negOne =>
+    { toFSM := FSM.negOne,
+      good := by ext; simp [Term.evalFin] }
+  | Term.and t₁ t₂ =>
+    let q₁ := termEvalEqFSM t₁
+    let q₂ := termEvalEqFSM t₂
+    { toFSM := composeBinary FSM.and q₁ q₂,
+      good := by ext; simp }
+  | Term.or t₁ t₂ =>
+    let q₁ := termEvalEqFSM t₁
+    let q₂ := termEvalEqFSM t₂
+    { toFSM := composeBinary FSM.or q₁ q₂,
+      good := by ext; simp }
+  | Term.xor t₁ t₂ =>
+    let q₁ := termEvalEqFSM t₁
+    let q₂ := termEvalEqFSM t₂
+    { toFSM := composeBinary FSM.xor q₁ q₂,
+      good := by ext; simp }
+  | ls b t =>
+    let q := termEvalEqFSM t
+    { toFSM := by dsimp [arity]; exact composeUnary (FSM.ls b) q,
+      good := by ext; simp }
+  | Term.not t =>
+    let q := termEvalEqFSM t
+    { toFSM := by dsimp [arity]; exact composeUnary FSM.not q,
+      good := by ext; simp }
+  | add t₁ t₂ =>
+    let q₁ := termEvalEqFSM t₁
+    let q₂ := termEvalEqFSM t₂
+    { toFSM := composeBinary FSM.add q₁ q₂,
+      good := by ext; simp }
+  | sub t₁ t₂ =>
+    let q₁ := termEvalEqFSM t₁
+    let q₂ := termEvalEqFSM t₂
+    { toFSM := composeBinary FSM.sub q₁ q₂,
+      good := by ext; simp }
+  | neg t =>
+    let q := termEvalEqFSM t
+    { toFSM := by dsimp [arity]; exact composeUnary FSM.neg q,
+      good := by ext; simp }
+  | incr t =>
+    let q := termEvalEqFSM t
+    { toFSM := by dsimp [arity]; exact composeUnary FSM.incr q,
+      good := by ext; simp }
+  | decr t =>
+    let q := termEvalEqFSM t
+    { toFSM := by dsimp [arity]; exact composeUnary FSM.decr q,
+      good := by ext; simp }
 
-variable
-  (init_carry : α → Bool)
-  (next_carry : ∀ (_carry : α → Bool) (_bits : β → Bool), (α → Bool))
-  (next_bit : ∀ (_carry : α → Bool) (_bits : β → Bool), (α → Bool) × Bool)
-
-variable [Fintype α] [Fintype α']
-
-open Fintype
-
-lemma exists_repeat_carry (seq : β → ℕ → Bool) :
-    ∃ n m : Fin (2 ^ (card α) + 1),
-      propagateCarry2 init_carry next_carry seq n =
-      propagateCarry2 init_carry next_carry seq m ∧
-      n < m := by
-  by_contra h
-  haveI := Classical.decEq α
-  push_neg at h
-  have := λ a b hab => (le_antisymm (h a b hab) (h b a hab.symm)).symm
-  have := Fintype.card_le_of_injective _ this
-  simp at this
-
-lemma propagateCarry2_eq_of_seq_eq_lt (seq₁ seq₂ : β → ℕ → Bool)
-    (init_carry : α → Bool)
-    (next_carry : ∀ (_carry : α → Bool) (_bits : β → Bool), (α → Bool))
-    (i : ℕ) (h : ∀ (b) (j) (_hj : j < i), seq₁ b j = seq₂ b j) :
-    propagateCarry2 init_carry next_carry seq₁ i =
-      propagateCarry2 init_carry next_carry seq₂ i := by
-  induction' i with i ih
-  { simp [propagateCarry2] }
-  { simp only [propagateCarry2, h _ i (Nat.lt_succ_self i)]
-    rw [ih]
-    exact λ b j hj => h b j (Nat.lt_succ_of_lt hj) }
-
-lemma propagate_eq_of_seq_eq_le (seq₁ seq₂ : β → ℕ → Bool)
-    (init_carry : α → Bool)
-    (next_bit : ∀ (_carry : α → Bool) (_bits : β → Bool), (α → Bool) × Bool)
-    (i : ℕ) (h : ∀ (b) (j) (_hj : j ≤ i), seq₁ b j = seq₂ b j) :
-    propagate init_carry next_bit seq₁ i =
-      propagate init_carry next_bit seq₂ i := by
-  cases i
-  { simp [propagate_zero, h _ 0 (le_refl _)] }
-  { simp only [propagate_succ2, propagate_succ2, h _ _ (le_refl _)]
-    congr 2
-    apply propagateCarry2_eq_of_seq_eq_lt
-    exact λ b j hj => h b j (le_of_lt hj) }
-
-
-lemma propagateCarry2_eq_of_carry_eq (seq₁ seq₂ : β → ℕ → Bool)
-    (m n : ℕ)
-    (h₁ : propagateCarry2 init_carry
-      (λ carry bits => (next_bit carry bits).1) seq₁ m =
-        propagateCarry2 init_carry
-      (λ carry bits => (next_bit carry bits).1) seq₂ n) (x : ℕ)
-    (h₃ : ∀ y b, y ≤ x → seq₁ b (m + y) = seq₂ b (n + y))  :
-    propagateCarry2 init_carry
-      (λ carry bits => (next_bit carry bits).1) seq₁ (m + x) =
-    propagateCarry2 init_carry
-      (λ carry bits => (next_bit carry bits).1) seq₂ (n + x) := by
-  induction' x with x ih generalizing seq₁ seq₂
-  { simp [*] at * }
-  { simp only [propagateCarry2, Nat.add_eq, h₃ x _ (Nat.le_succ _)] at *
-    rw [ih]
-    assumption
-    exact λ y b h => h₃ y b (Nat.le_succ_of_le h) }
-
-lemma propagate_eq_of_carry_eq (seq₁ seq₂ : β → ℕ → Bool)
-    (m n : ℕ)
-    (h₁ : propagateCarry2 init_carry
-      (λ carry bits => (next_bit carry bits).1) seq₁ m =
-        propagateCarry2 init_carry
-      (λ carry bits => (next_bit carry bits).1) seq₂ n) (x : ℕ)
-    (h₃ : ∀ y b, y ≤ x → seq₁ b (m + y) = seq₂ b (n + y))  :
-    propagate init_carry next_bit seq₁ (m + x) =
-    propagate init_carry next_bit seq₂ (n + x) := by
-  cases x
-  { cases m
-    { cases n
-      { simp [h₃ 0 _ (le_refl _), propagateCarry2, *] at * }
-      { simp [*, h₃ 0 _ (le_refl _), propagate_succ2] at *
-        rw [← h₁] } }
-    { cases n
-      { simp [*, propagate_succ2] at *
-        have := fun i => h₃ 0 i rfl
-        dsimp at this
-        simp [this]
-        simp [h₁] }
-      { rw [propagate_succ2, h₁, propagate_succ2]
-        have := h₃ 0
-        simp [*] at * } } }
-  { erw [Nat.add_succ, propagate_succ2, propagate_succ2, Nat.add_eq]
-    simp [← Nat.succ_eq_add_one, ← Nat.add_succ, h₃ _ _ (le_refl _)]
-    congr
-    . apply propagateCarry2_eq_of_carry_eq
-      . assumption
-      . exact λ y b h => h₃ y b (Nat.le_succ_of_le h)
-    . funext i
-      rw [h₃]
-      exact Nat.le_succ _ }
-
-lemma propagateCarry_propagateCarry_add (x : β → ℕ → Bool) :
-    ∀ (init_carry : α → Bool)
-      (next_carry : ∀ (_carry : α → Bool) (_bits : β → Bool), (α → Bool)),
-    ∀ n i : ℕ,
-    propagateCarry2 (propagateCarry2 init_carry next_carry x n)
-      next_carry (λ b k => x b (k + n)) i =
-    propagateCarry2 init_carry next_carry x (i + n)
-  | init_carry, _next_carry, 0, 0 => by simp [propagateCarry2]
-  | init_carry, next_carr, n+1, 0 =>
-    by simp [propagateCarry, propagateCarry2_succ]
-  | init_carry, next_carry, n, i+1 => by
-    rw [propagateCarry2, add_assoc,
-      propagateCarry_propagateCarry_add _ _ _ _ i]
-    simp only [Nat.one_add, Nat.add_one, Nat.succ_add, Nat.add_succ,
-      add_zero, propagateCarry2, zero_add]
-
-lemma exists_repeat : ∀ (seq : β → ℕ → Bool)
-    (n : ℕ),
-    ∃ (m : ℕ) (_hm : m < 2 ^ (card α)) (seq2 : β → ℕ → Bool),
-      propagate init_carry next_bit seq2 m = propagate init_carry next_bit seq n
-  | seq, n => by
-    by_cases hn2 : n < 2 ^ card α
-    { exact ⟨n, hn2, seq, rfl⟩ }
-    { rcases exists_repeat_carry
-        (propagateCarry2 init_carry (λ c b => (next_bit c b).1) seq
-          (n - 2 ^ card α))
-        (λ carry bits => (next_bit  carry bits).1)
-        (λ b i => seq b (i + (n - 2^ (card α)))) with ⟨a, b, h₁, h₂⟩
-      simp only [propagateCarry_propagateCarry_add] at h₁
-      rcases have _wf : n - (b - a) < n :=
-         Nat.sub_lt (lt_of_lt_of_le (pow_pos (by norm_num) _) (le_of_not_lt hn2)) (Nat.sub_pos_of_lt h₂)
-        exists_repeat (λ c i => if i < a + (n - 2 ^ card α) then seq c i else
-          seq c (i + (b - a))) (n - (b - a)) with ⟨m, hmle, seq2, hm⟩
-      use m; use hmle; use seq2
-      rw [hm]; clear hm
-      have h1 : n - (b - a) = (a + (n - 2 ^ (card α))) + (2 ^ card α - b) := by
-      { zify
-        rw [Nat.cast_sub, Nat.cast_sub, Nat.cast_sub, Nat.cast_sub]
-        ring_nf
-        exact Nat.le_of_lt_succ b.2
-        simp [*] at *
-        exact hn2
-        exact le_of_lt h₂
-        exact le_trans (Nat.sub_le _ _) (le_trans (Nat.le_of_lt_succ b.2)
-          (le_of_not_lt hn2)) }
-      rw [h1]
-      have h2 : n = (b + (n - 2 ^ card α)) + (2 ^ card α - b) := by
-      { zify
-        rw [Nat.cast_sub, Nat.cast_sub]
-        ring
-        exact Nat.le_of_lt_succ b.2
-        simp [*] at *
-        exact hn2 }
-      conv_rhs => rw [h2]
-      refine' propagate_eq_of_carry_eq _ _ _ _ _ _ _ _ _
-      { have _h : ↑b + (n - 2 ^ card α) = (a + (n - 2 ^ card α)) + (b - a) := by
-        { zify
-          rw [Nat.cast_sub, Nat.cast_sub]
-          ring_nf
-          exact le_of_lt h₂
-          exact le_of_not_lt hn2 }
-        rw [← h₁]
-        apply propagateCarry2_eq_of_seq_eq_lt
-        simp (config := { contextual := true }) }
-      { intro y c _hc
-        simp only [add_lt_iff_neg_left, not_lt_zero', if_false]
-        congr 1
-        zify
-        rw [Nat.cast_sub, Nat.cast_sub]
-        ring
-        exact le_of_lt h₂
-        exact le_of_not_lt hn2 } }
-
-
-lemma propagate_eq_zero_iff (init_carry : α → Bool)
-    (next_bit : ∀ (_carry : α → Bool) (_bits : β → Bool), (α → Bool) × Bool) :
-    (∀ seq, propagate init_carry next_bit seq = zeroSeq) ↔
-    (∀ seq, ∀ i < 2 ^ (card α), propagate init_carry next_bit seq i = false) := by
-  constructor
-  { intro h i _
-    simp [h, zeroSeq] }
-  { intro h seq
-    funext i
-    rcases exists_repeat init_carry next_bit seq i with ⟨j, hj, seq2, hseq2⟩
-    rw [← hseq2, h seq2 j hj, zeroSeq] }
-
-lemma eq_iff_xorSeq_eq_zero (seq₁ seq₂ : ℕ → Bool) :
-    (∀ i, seq₁ i = seq₂ i) ↔ (∀ i, xorSeq seq₁ seq₂ i = zeroSeq i) := by
-  simp [Function.funext_iff, xorSeq, zeroSeq]
-  constructor
-  { intro i _; simp [*] }
-  { intro h a
-    specialize h a
-    revert h
-    cases (seq₁ a) <;> cases (seq₂ a) <;> simp [*] at * }
-
-lemma eval_eq_iff_xorSeq_eq_zero (t₁ t₂ : Term) :
-    t₁.eval = t₂.eval ↔ (t₁.xor t₂).evalFin = λ _ => zeroSeq := by
-  simp only [Function.funext_iff, Term.eval, Term.evalFin,
-    ← eq_iff_xorSeq_eq_zero, ← evalFin_eq_eval]
-  constructor
-  { intro h seq n
-    have := h (λ j => if hj : j < (arity (t₁.xor t₂)) then seq ⟨j, hj⟩ else λ _ => false) n
-    simp at this
-    convert this using 1 }
-  { intro h seq m
-    exact h (λ j => seq j) _ }
